Improved wcbvEval relation in extraction. Avoids all unnecessary uses of mkApps

extraction/theories/EWcbvEval.v
@@ -2,11 +2,13 @@
 
 From Coq Require Import Bool String List Program BinPos Compare_dec Omega.
 From MetaCoq.Template Require Import config utils Ast.
-From MetaCoq.Extraction Require Import EAst EInduction ELiftSubst ETyping.
+From MetaCoq.PCUIC Require Import PCUICAstUtils.
+From MetaCoq.Extraction Require Import EAst EAstUtils EInduction ELiftSubst ETyping Prelim.
 From MetaCoq.Template Require AstUtils.
 Require Import String.
 Local Open Scope string_scope.
 Set Asymmetric Patterns.
+Require Import ssreflect ssrbool.
 
 Existing Instance config.default_checker_flags.
 
@@ -29,8 +31,218 @@ Definition atom t :=
   match t with
   | tBox
   | tConstruct _ _
-  | tFix _ _
+  | tCoFix _ _
+  | tLambda _ _
+  | tFix _ _ => true
+  | _ => false
+  end.
+
+Lemma mkApps_app t l l' : mkApps t (l ++ l') = mkApps (mkApps t l) l'.
+Proof.
+  induction l in t, l' |- *; simpl; auto.
+Qed.
+
+Lemma decompose_app_rec_inv {t l' f l} :
+  decompose_app_rec t l' = (f, l) ->
+  mkApps t l' = mkApps f l.
+Proof.
+  induction t in f, l', l |- *; try intros [= <- <-]; try reflexivity.
+  simpl. apply/IHt1.
+Qed.
+
+Lemma decompose_app_inv {t f l} :
+  decompose_app t = (f, l) -> t = mkApps f l.
+Proof. by apply/decompose_app_rec_inv. Qed.
+Lemma atom_decompose_app t l : ~~ isApp t -> decompose_app_rec t l = pair t l.
+Proof. destruct t; simpl; congruence. Qed.
+
+Lemma mkApps_eq_decompose_app_rec {f args t l} :
+  mkApps f args = t ->
+  ~~ isApp f ->
+  match decompose_app_rec t l with
+  | (f', args') => f' = f /\ mkApps t l = mkApps f' args'
+  end.
+Proof.
+  revert f t l.
+  induction args using rev_ind; simpl.
+  - intros * -> **. rewrite atom_decompose_app; auto.
+  - intros. rewrite mkApps_app in H.
+    specialize (IHargs f).
+    destruct (isApp t) eqn:Heq.
+    destruct t; try discriminate.
+    simpl in Heq. inv H. simpl.
+    specialize (IHargs (mkApps f args) (t2 :: l) eq_refl H0).
+    destruct decompose_app_rec. intuition.
+    subst t.
+    simpl in Heq. discriminate.
+Qed.
+
+Lemma decompose_app_eq_right t l l' : decompose_app_rec t l = decompose_app_rec t l' -> l = l'.
+Proof.
+  induction t in l, l' |- *; simpl; intros [=]; auto.
+  specialize (IHt1 _ _ H0). now inv IHt1.
+Qed.
+
+Lemma mkApps_eq_right t l l' : mkApps t l = mkApps t l' -> l = l'.
+Proof.
+  intros. eapply (f_equal decompose_app) in H. unfold decompose_app in H.
+  rewrite !decompose_app_rec_mkApps in H. apply decompose_app_eq_right in H.
+  now rewrite !app_nil_r in H.
+Qed.
+
+Lemma mkApps_eq_decompose' {f args t} :
+  mkApps f args = t ->
+  ~~ isApp f ->
+  match decompose_app t with
+  | (f', args') => f' = f /\ args' = args /\ t = mkApps f' args'
+  end.
+Proof.
+  intros.
+  have H' := (@mkApps_eq_decompose_app_rec f args t [] H H0).
+  rewrite /decompose_app. destruct (decompose_app_rec t []).
+  intuition subst; auto. simpl in H2. now eapply mkApps_eq_right in H2.
+Qed.
+
+
+Lemma decompose_app_rec_notApp :
+  forall t l u l',
+    decompose_app_rec t l = (u, l') ->
+    ~~ isApp u.
+Proof.
+  intros t l u l' e.
+  induction t in l, u, l', e |- *.
+  all: try (cbn in e ; inversion e ; reflexivity).
+  cbn in e. eapply IHt1. eassumption.
+Qed.
+
+Lemma decompose_app_notApp :
+  forall t u l,
+    decompose_app t = (u, l) ->
+    ~~ isApp u.
+Proof.
+  intros t u l e.
+  eapply decompose_app_rec_notApp. eassumption.
+Qed.
+
+Inductive mkApps_spec : term -> list term -> term -> list term -> term -> Type :=
+| mkApps_intro f l n :
+    ~~ isApp f ->
+    mkApps_spec f l (mkApps f (firstn n l)) (skipn n l) (mkApps f l).
+
+Lemma decompose_app_rec_eq f l :
+  ~~ isApp f ->
+  decompose_app_rec f l = (f, l).
+Proof.
+  destruct f; simpl; try discriminate; congruence.
+Qed.
+Close Scope string_scope.
+
+Lemma firstn_add {A} x y (args : list A) : firstn (x + y) args = firstn x args ++ firstn y (skipn x args).
+Proof.
+  induction x in y, args |- *. simpl. reflexivity.
+  simpl. destruct args. simpl.
+  now rewrite skipn_nil firstn_nil.
+  rewrite IHx. now rewrite app_comm_cons.
+Qed.
+
+Lemma decompose_app_rec_inv' f l hd args :
+  decompose_app_rec f l = (hd, args) ->
+  ∑ n, ~~ isApp hd /\ l = skipn n args /\ f = mkApps hd (firstn n args).
+Proof.
+  destruct (isApp f) eqn:Heq.
+  revert l args hd.
+  induction f; try discriminate. intros.
+  simpl in H.
+  destruct (isApp f1) eqn:Hf1.
+  2:{ rewrite decompose_app_rec_eq in H => //. now apply negbT.
+      inv H. exists 1. simpl. intuition auto. now eapply negbT. }
+  destruct (IHf1 eq_refl _ _ _ H).
+  clear IHf1.
+  exists (S x); intuition auto. eapply (f_equal (skipn 1)) in H2.
+  rewrite [l]H2. now rewrite skipn_skipn Nat.add_1_r.
+  rewrite -Nat.add_1_r firstn_add H3 -H2.
+  now rewrite -[tApp _ _](mkApps_app hd _ [f2]).
+  rewrite decompose_app_rec_eq; auto. now apply negbT.
+  move=> [] H ->. subst f. exists 0. intuition auto.
+  now apply negbT.
+Qed.
+
+Lemma mkApps_elim_rec t l l' :
+  let app' := decompose_app_rec (mkApps t l) l' in
+  mkApps_spec app'.1 app'.2 t (l ++ l') (mkApps t (l ++ l')).
+Proof.
+  destruct app' as [hd args] eqn:Heq.
+  subst app'.
+  rewrite decompose_app_rec_mkApps in Heq.
+  have H := decompose_app_rec_inv' _ _ _ _ Heq.
+  destruct H. simpl. destruct a as [isapp [Hl' Hl]].
+  subst t.
+  have H' := mkApps_intro hd args x. rewrite Hl'.
+  rewrite -mkApps_app. now rewrite firstn_skipn.
+Qed.
+
+Lemma mkApps_elim t l  :
+  let app' := decompose_app (mkApps t l) in
+  mkApps_spec app'.1 app'.2 t l (mkApps t l).
+Proof.
+  have H := @mkApps_elim_rec t l [].
+  now rewrite app_nil_r in H.
+Qed.
+
+Lemma mkApps_eq_inj {t t' l l'} :
+  mkApps t l = mkApps t' l' ->
+  ~~ isApp t -> ~~ isApp t' -> t = t' /\ l = l'.
+Proof.
+  intros Happ Ht Ht'. eapply (f_equal decompose_app) in Happ. unfold decompose_app in Happ.
+  rewrite !decompose_app_rec_mkApps in Happ. rewrite !atom_decompose_app in Happ; auto.
+  now rewrite !app_nil_r in Happ.
+Qed.
+
+Ltac solve_discr :=
+  match goal with
+    H : mkApps _ _ = mkApps ?f ?l |- _ =>
+    eapply mkApps_eq_inj in H as [? ?]; [|easy|easy]; subst; try intuition congruence
+  | H : ?t = mkApps ?f ?l |- _ =>
+    change t with (mkApps t []) in H ;
+    eapply mkApps_eq_inj in H as [? ?]; [|easy|easy]; subst; try intuition congruence
+  | H : mkApps ?f ?l = ?t |- _ =>
+    change t with (mkApps t []) in H ;
+    eapply mkApps_eq_inj in H as [? ?]; [|easy|easy]; subst; try intuition congruence
+  end.
+
+Lemma atom_mkApps f l : atom (mkApps f l) -> (l = []) /\ atom f.
+Proof.
+  revert f; induction l using rev_ind. simpl. intuition auto.
+  simpl. intros. now rewrite mkApps_app in H.
+Qed.
+
+Definition isEvar t :=
+  match t with
+  | tEvar _ _ => true
+  | _ => false
+  end.
+
+Definition isFix t :=
+  match t with
+  | tFix _ _ => true
+  | _ => false
+  end.
+
+Definition isCoFix t :=
+  match t with
   | tCoFix _ _ => true
+  | _ => false
+  end.
+
+Definition isConstruct t :=
+  match t with
+  | tConstruct _ _ => true
+  | _ => false
+  end.
+
+Definition isBox t :=
+  match t with
+  | tBox => true
   | _ => false
   end.
 
@@ -40,9 +252,10 @@ Section Wcbv.
 
   Inductive eval : term -> term -> Prop :=
   (** Reductions *)
-  | eval_box a l :
+  | eval_box a t t' :
       eval a tBox ->
-      eval (tApp a l) tBox
+      eval t t' ->
+      eval (tApp a t) tBox
 
   (** Beta *)
   | eval_beta f na b a a' res :
@@ -70,16 +283,15 @@ Section Wcbv.
       eval (mkApps f (repeat tBox n)) res ->
       eval (tCase (ind, pars) discr brs) res
            
-  (** Fix unfolding, with guard *)
-  | eval_fix mfix idx args args' narg fn res :
+  (** Fix unfolding, without guard *)
+  | eval_fix mfix idx arg narg fn res :
       unfold_fix mfix idx = Some (narg, fn) ->
       (* We do not need to check the guard in the extracted language
          as we assume reduction of closed terms, whose canonical
-         form will be a constructor or a box.  *)
-      (* is_constructor_or_box narg args' -> *)
-      Forall2 eval args args' ->
-      eval (mkApps fn args') res ->
-      eval (mkApps (tFix mfix idx) args) res
+         form will be a constructor or a box. A fixpoint must
+         still be applied to at least one argument to unfold. *)
+      eval (tApp fn arg) res ->
+      eval (tApp (tFix mfix idx) arg) res
 
   (** CoFix-case unfolding *)
   | red_cofix_case ip mfix idx args narg fn brs res :
@@ -109,157 +321,319 @@ Section Wcbv.
   | eval_proj_box i pars arg discr :
       eval discr tBox ->
       eval (tProj (i, pars, arg) discr) tBox
-           
-  (** Abstractions are values *)
-  | eval_abs na N : eval (tLambda na N) (tLambda na N)
 
-  (** Constructors applied to values are values *)
-  | eval_constr f i k l l' :
-      eval f (tConstruct i k) ->
-      Forall2 eval l l' ->
-      eval (mkApps f l) (mkApps (tConstruct i k) l')
+  (** Atoms (non redex-producing heads) applied to values are values *)
+  | eval_app_cong f f' a a' :
+      eval f f' ->
+      ~~ (isLambda f' || isFix f' || isBox f') ->
+      eval a a' ->
+      eval (tApp f a) (tApp f' a')
 
-  (** Atoms are values *)
-  | eval_atom t : atom t -> eval t t
+  (** Evars complicate reasoning due to the embedded substitution, we skip
+      them for now *)
+  (* | eval_evar n l l' : *)
+  (*     Forall2 eval l l' -> *)
+  (*     eval (tEvar n l) (tEvar n l') *)
 
-  | eval_evar ev l : eval (tEvar ev l) (tEvar ev l) (* Lets say it is a value for now *).
 
-  (* (** The right induction principle for the nested [Forall] cases: *) *)
+  (** Atoms are values (includes abstractions, cofixpoints and constructors) *)
+  | eval_atom t : atom t -> eval t t.
 
-  Lemma eval_evals_ind :
-    forall P : term -> term -> Prop,
-      (forall a l, eval a tBox ->
-                   P (tApp a l) tBox) ->
-      (forall (f : term) (na : name) (b a a' : term) (res : term),
-          eval f (tLambda na b) ->
-          P f (tLambda na b) ->
-          eval a a' -> P a a' ->
-          eval (b {0 := a'}) res -> P (b {0 := a'}) res -> P (tApp f a) res) ->
+  (** Characterization of values for this reduction relation.
+      Only constructors and cofixpoints can accumulate arguments.
+      All other values are atoms and cannot have arguments:
+      - box
+      - abstractions
+      - constant constructors
+      - unapplied fixpoints and cofixpoints
+   *)
 
-      (forall (na : name) (b0 b0' b1 res : term),
-          eval b0 b0' -> P b0 b0' -> eval (b1 {0 := b0'}) res -> P (b1 {0 := b0'}) res ->
-          P (tLetIn na b0 b1) res) ->
-
-      (forall (ind : inductive) (pars : nat) (discr : term) (c : nat)
-              (args : list term) (brs : list (nat * term)) (res : term),
-          eval discr (mkApps (tConstruct ind c) args) ->
-          P discr (mkApps (tConstruct ind c) args) ->
-          eval (iota_red pars c args brs) res ->
-          P (iota_red pars c args brs) res -> P (tCase (ind, pars) discr brs) res) ->
-
-      (forall (ind : inductive) (pars : nat) (discr : term) (brs : list (nat * term)) (n : nat) (f3 res : term),
-        eval discr tBox ->
-        P discr tBox ->
-        brs = [(n, f3)] ->
-        eval (mkApps f3 (repeat tBox n)) res ->
-        P (mkApps f3 (repeat tBox n)) res -> P (tCase (ind, pars) discr brs) res) ->
-      
-      (forall (mfix : mfixpoint term) (idx : nat) (args args' : list term) (narg : nat) (fn res : term),
-          unfold_fix mfix idx = Some (narg, fn) ->
-          Forall2 eval args args' ->
-          Forall2 P args args' ->
-          (* is_constructor_or_box narg args' = true -> *)
-          eval (mkApps fn args') res -> P (mkApps fn args') res -> P (mkApps (tFix mfix idx) args) res) ->
-
-      (forall (ip : inductive * nat)  (mfix : mfixpoint term) (idx : nat) (args : list term)
-              (narg : nat) (fn : term) (brs : list (nat * term)) (res : term),
-          unfold_cofix mfix idx = Some (narg, fn) ->
-          eval (tCase ip (mkApps fn args) brs) res ->
-          P (tCase ip (mkApps fn args) brs) res -> P (tCase ip (mkApps (tCoFix mfix idx) args) brs) res) ->
-
-      (forall (p : projection) (mfix : mfixpoint term) (idx : nat) (args : list term) (narg : nat) (fn res : term),
-          unfold_cofix mfix idx = Some (narg, fn) ->
-          eval (tProj p (mkApps fn args)) res ->
-          P (tProj p (mkApps fn args)) res -> P (tProj p (mkApps (tCoFix mfix idx) args)) res) ->
-
-      (forall (c : ident) (decl : constant_body) (body : term),
-          declared_constant Σ c decl ->
-          forall (res : term),
-            cst_body decl = Some body ->
-            eval body res -> P body res -> P (tConst c) res) ->
-
-      (forall (i : inductive) (pars arg : nat) (discr : term) (args : list term) (k : nat)
-              (res : term),
-          eval discr (mkApps (tConstruct i k) args) ->
-          P discr (mkApps (tConstruct i k) args) ->
-          eval (nth (pars + arg) args tDummy) res ->
-          P (nth (pars + arg) args tDummy) res -> P (tProj (i, pars, arg) discr) res) ->
-
-      (forall (i : inductive) (pars arg : nat) (discr : term),
-          eval discr tBox ->
-          P discr tBox ->
-          P (tProj (i, pars, arg) discr) tBox) ->
-      
-      (forall (na : name) (M N : term), P (tLambda na N) (tLambda na N)) ->
-
-      (forall (f8 : term) (i : inductive) (k : nat) (l l' : list term),
-          eval f8 (tConstruct i k) ->
-          P f8 (tConstruct i k) -> Forall2 eval l l' -> Forall2 P l l' -> P (mkApps f8 l) (mkApps (tConstruct i k) l')) ->
-      (forall t, atom t -> P t t) ->
-
-      (forall (ev : nat) (l : list term), P (tEvar ev l) (tEvar ev l)) ->
-
-      forall t t0 : term, eval t t0 -> P t t0.
-  Proof.
-    intros P Hbox Hbeta Hlet Hcase Hscase Hfix Hcoficase Hcofixproj
-           Hconst Hproj Hproj2 Hlam Hcstr Hatom Hevar.
-    fix eval_evals_ind 3. destruct 1;
-             try match goal with [ H : _ |- _ ] =>
-                             match type of H with
-                               forall t t0, eval t t0 -> _ => fail 1
-                             | context [ atom _ ] => fail
-                             | _ => try solve [eapply H; eauto]
-                             end end; eauto.
-    eapply Hfix. eauto. eauto.
-    clear H1.
-    revert args args' H0. fix aux 3. destruct 1. constructor; auto.
-    constructor. now apply eval_evals_ind. now apply aux. all:eauto.
-    eapply Hcstr; eauto.
-    revert l l' H0. fix aux 3. destruct 1; constructor.
-    now apply eval_evals_ind. apply aux. auto.
-  Defined.
-
-  (** Characterization of values for this reduction relation: *)
-  (*     Basically atoms (constructors, inductives, products (FIXME sorts missing)) *)
-  (*     and de Bruijn variables and lambda abstractions. Closed values disallow *)
-  (*     de Bruijn variables. *)
+  Definition value_head x :=
+    isConstruct x || isCoFix x.
 
   Inductive value : term -> Prop :=
   | value_atom t : atom t -> value t
-  | value_tEvar ev l : value (tEvar ev l)
-  | value_tLam na b : value (tLambda na b)
-  | value_tConstructApp i k l : Forall value l -> value (mkApps (tConstruct i k) l).
+  (* | value_evar n l l' : Forall value l -> Forall value l' -> value (mkApps (tEvar n l) l') *)
+  | value_app t l : value_head t -> Forall value l -> value (mkApps t l).
 
   Lemma value_values_ind : forall P : term -> Prop,
       (forall t, atom t -> P t) ->
-      (forall (ev : nat) (l : list term), P (tEvar ev l)) ->
-      (forall (na : name) (b : term), P (tLambda na b)) ->
-      (forall (i : inductive) (k : nat) (l : list term),
-          Forall value l -> Forall P l -> P (mkApps (tConstruct i k) l)) ->
+      (* (forall n l l', Forall value l -> Forall P l -> Forall value l' -> Forall P l' -> *)
+      (*                 P (mkApps (tEvar n l) l')) -> *)
+      (forall t l, value_head t -> Forall value l -> Forall P l -> P (mkApps t l)) ->
       forall t : term, value t -> P t.
   Proof.
-    intros P ????.
-    fix value_values_ind 2. destruct 1. 1-3:clear value_values_ind; auto.
-    apply H2; auto.
-    revert l H3. fix aux 2. destruct 1. constructor; auto.
-    constructor. now apply value_values_ind. now apply aux.
+    intros P ??.
+    fix value_values_ind 2. destruct 1. apply H; auto.
+    eapply H0; auto.
+    revert l H2. fix aux 2. destruct 1. constructor; auto.
+    constructor. now eapply value_values_ind. now apply aux.
   Defined.
+
+  Lemma value_head_nApp t : value_head t -> ~~ isApp t.
+  Proof. destruct t; auto. Qed.
+  Hint Resolve value_head_nApp : core.
+
+  Lemma value_mkApps_inv t l :
+    ~~ isApp t ->
+    value (mkApps t l) ->
+    (l = [] /\ atom t) \/ (value_head t /\ Forall value l).
+  Proof.
+    intros H H'. generalize_eqs H'. revert t H. induction H' using value_values_ind.
+    intros.
+    subst.
+    - now eapply atom_mkApps in H.
+    - intros * isapp appeq. solve_discr.
+  Qed.
 
   (** The codomain of evaluation is only values: *)
   (*     It means no redex can remain at the head of an evaluated term. *)
 
-  Lemma eval_to_value e e' : eval e e' -> value e'.
+  Lemma Forall_skipn {A} (P : A -> Prop) n l : Forall P l -> Forall P (skipn n l).
   Proof.
-    induction 1 using eval_evals_ind; simpl; auto using value.
-    eapply (value_tConstructApp i k).
-    apply (Forall2_right _ _ _ H1).
+    intros H. revert n; induction H; intros n. rewrite skipn_nil; auto.
+    destruct n; simpl.
+    - rewrite /skipn. constructor; auto.
+    - now rewrite skipn_S.
   Qed.
 
-  (** Evaluation preserves closedness: *)
-  Lemma eval_closed : forall n t u, closedn n t = true -> eval t u -> closedn n u = true.
+  Lemma Forall_firstn {A} (P : A -> Prop) n l : Forall P l -> Forall P (firstn n l).
   Proof.
-    induction 2 using eval_evals_ind; simpl in *; auto. eapply IHeval3.
-    admit.
-  Admitted. (* closedness of evaluates for Eterms, not needed for verification *)
+    intros H. revert n; induction H; intros n. rewrite firstn_nil; auto.
+    destruct n; simpl.
+    - constructor; auto.
+    - constructor; auto.
+  Qed.
+
+  Lemma value_head_spec t :
+    value_head t = (~~ (isLambda t || isFix t || isBox t)) && atom t.
+  Proof.
+    destruct t; intuition auto.
+  Qed.
+
+  Lemma eval_to_value e e' : eval e e' -> value e'.
+  Proof.
+    induction 1 using eval_ind; simpl; auto using value.
+    (* eapply (value_app (tEvar n l') []). constructor. constructor. *)
+    destruct (mkApps_elim f' []).
+    eapply value_mkApps_inv in IHeval1.
+    destruct IHeval1; intuition subst.
+    rewrite H3.
+    simpl. rewrite H3 in H0. simpl in *.
+    apply (value_app f0 [a']).
+    rewrite value_head_spec. now rewrite H0 H4.
+    constructor; auto.
+    rewrite -[tApp _ _](mkApps_app _ (firstn n l) [a']).
+    constructor 2; auto. eapply app_Forall; auto. auto.
+  Qed.
+
+  Lemma Forall2_app_r {A} (P : A -> A -> Prop) l l' r r' : Forall2 P (l ++ [r]) (l' ++ [r']) ->
+                                                           (Forall2 P l l') * (P r r').
+  Proof.
+    induction l in l', r |- *. simpl. intros. destruct l'. simpl in *.
+    depelim H; intuition auto.
+    depelim H. destruct l'; depelim H0.
+    intros.
+    depelim l'; depelim H. destruct l; depelim H0.
+    specialize (IHl _ _ H0). intuition auto.
+  Qed.
+
+  Lemma value_final e : value e -> eval e e.
+  Proof.
+    induction 1 using value_values_ind; simpl; auto using value.
+    now constructor.
+    assert (Forall2 eval l l).
+    induction H1; constructor; auto. eapply IHForall. now depelim H0.
+    rewrite value_head_spec in H.
+    induction l using rev_ind. simpl.
+    move/andP: H => [H H'].
+    constructor; try easy.
+    rewrite mkApps_app.
+    eapply Forall_app in H0 as [Hl Hx]. depelim Hx.
+    eapply Forall2_app_r in H2 as [Hl' Hx'].
+    eapply eval_app_cong; auto.
+    eapply IHl. auto.
+    now eapply Forall2_Forall. auto.
+    move/andP: H => [Ht Ht'].
+    destruct l using rev_ind; auto. now rewrite mkApps_app; simpl.
+  Qed.
+
+  (* (** Evaluation preserves closedness: *) *)
+  (* Lemma eval_closed : forall n t u, closedn n t = true -> eval t u -> closedn n u = true. *)
+  (* Proof. *)
+  (*   induction 2 using eval_ind; simpl in *; auto. eapply IHeval3. *)
+  (*   admit. *)
+  (* Admitted. (* closedness of evaluates for Eterms, not needed for verification *) *)
+
+  Lemma eval_tApp_tFix_inv mfix idx a v :
+    eval (tApp (tFix mfix idx) a) v ->
+    (exists fn arg,
+        (unfold_fix mfix idx = Some (arg, fn)) /\
+        (eval (tApp fn a) v)).
+  Proof.
+    intros H; depind H; try solve_discr.
+    - depelim H.
+    - depelim H.
+    - eexists _, _; firstorder eauto.
+    - now depelim H.
+    - discriminate.
+  Qed.
+
+  Lemma eval_tBox t : eval tBox t -> t = tBox.
+  Proof.
+    intros H; depind H; try solve_discr. auto.
+  Qed.
+
+  Lemma eval_tRel n t : eval (tRel n) t -> False.
+  Proof.
+    intros H; depind H; try solve_discr; try now easy.
+  Qed.
+
+  Lemma eval_tVar i t : eval (tVar i) t -> False.
+  Proof.
+    intros H; depind H; try solve_discr; try now easy.
+  Qed.
+
+  Lemma eval_tEvar n l t : eval (tEvar n l) t -> False.
+                          (* exists l', Forall2 eval l l' /\ (t = tEvar n l'). *)
+  Proof.
+    intros H; depind H; try solve_discr; try now easy.
+  Qed.
+
+  Lemma eval_atom_inj t t' : atom t -> eval t t' -> t = t'.
+  Proof.
+    intros Ha H; depind H; try solve_discr; try now easy.
+  Qed.
+
+  Lemma eval_LetIn {n b t v} :
+    eval (tLetIn n b t) v ->
+    exists b',
+      eval b b' /\ eval (t {0 := b'}) v.
+  Proof.
+    intros H; depind H; try solve_discr; try now easy.
+  Qed.
+
+  Lemma eval_Const {c v} :
+    eval (tConst c) v ->
+    exists decl body, declared_constant Σ c decl /\
+                      cst_body decl = Some body /\
+                      eval body v.
+  Proof.
+    intros H; depind H; try solve_discr; try now easy.
+    exists decl, body. intuition auto.
+  Qed.
+
+  Lemma eval_mkApps_tCoFix mfix idx l v :
+    eval (mkApps (tCoFix mfix idx) l) v ->
+    (exists l', Forall2 eval l l' /\ (v = mkApps (tCoFix mfix idx) l')).
+  Proof.
+    intros H.
+    depind H; try solve_discr.
+    destruct (mkApps_elim a [t]).
+    rewrite -[tApp _ _](mkApps_app f (firstn n l0) [t]) in x.
+    solve_discr.
+    specialize (IHeval1 _ _ _ eq_refl).
+    firstorder eauto.
+    solve_discr.
+    destruct (mkApps_elim f [a]).
+    rewrite -[tApp _ _](mkApps_app f (firstn n l0) [a]) in x. solve_discr.
+    specialize (IHeval1 _ _ _ eq_refl).
+    firstorder eauto. solve_discr.
+    change (tApp (tFix mfix0 idx0) arg) with (mkApps (tFix mfix0 idx0) [arg]) in x.
+    solve_discr.
+    change (tApp f a) with (mkApps f [a]) in x.
+    assert (l <> []).
+    destruct l; simpl in *; discriminate.
+    rewrite (app_removelast_last a H2) in x |- *.
+    rewrite mkApps_app in x. simpl in x. inv x.
+    specialize (IHeval1 _ _ _ eq_refl).
+    destruct IHeval1 as [l' [evl' eqf']].
+    exists (l' ++ [a']).
+    split. eapply Forall2_app; auto. constructor. now rewrite -!H5. constructor.
+    subst f'.
+    now rewrite mkApps_app.
+    eapply atom_mkApps in H; intuition try easy.
+    subst.
+    exists []. intuition auto.
+  Qed.
+
+  Lemma eval_deterministic {t v v'} : eval t v -> eval t v' -> v = v'.
+  Proof.
+    intros tv. revert v'.
+    revert t v tv.
+    induction 1 using eval_ind; intros v' tv'.
+    - depelim tv'; auto. specialize (IHtv1 _ tv'1); congruence.
+      depelim tv1. specialize (IHtv1 _ tv'1). now subst. easy.
+    - depelim tv'; auto; try specialize (IHtv1 _ tv'1) || solve [depelim tv1]; try congruence.
+      inv IHtv1. specialize (IHtv2 _ tv'2). subst.
+      now specialize (IHtv3 _ tv'3).
+      now subst f'. easy.
+    - eapply eval_LetIn in tv' as [b' [evb evt]].
+      rewrite -(IHtv1 _ evb) in evt.
+      eapply (IHtv2 _ evt).
+    - depelim tv'; try solve_discr.
+      * specialize (IHtv1 _ tv'1).
+        solve_discr. inv H.
+        now specialize (IHtv2 _ tv'2).
+      * specialize (IHtv1 _ tv'1); solve_discr.
+      * eapply eval_mkApps_tCoFix in tv1 as [l' [ev' eq]]. solve_discr.
+      * easy.
+    - subst.
+      depelim tv'.
+      * specialize (IHtv1 _ tv'1).
+        solve_discr.
+      * specialize (IHtv1 _ tv'1).
+        now specialize (IHtv2 _ tv'2).
+      * pose proof tv1. eapply eval_mkApps_tCoFix in H0.
+        destruct H0 as [l' [evargs eq]]. solve_discr.
+      * easy.
+    - depelim tv' => //.
+      * depelim tv'1.
+      * depelim tv'1.
+      * rewrite H in H0. inv H0.
+        now specialize (IHtv _ tv').
+      * now depelim tv'1.
+
+    - depelim tv'; try easy.
+      * eapply eval_mkApps_tCoFix in tv'1 as [l' [evargs eq]].
+        solve_discr.
+      * eapply eval_mkApps_tCoFix in tv'1 as [l' [evargs eq]].
+        solve_discr.
+      * solve_discr. inv H1. rewrite H in H0. inv H0.
+        now specialize (IHtv _ tv').
+
+    - depelim tv'; try easy.
+      * solve_discr. inv H1. rewrite H in H0. inv H0.
+        now specialize (IHtv _ tv').
+      * eapply eval_mkApps_tCoFix in tv'1 as [l' [evargs eq]].
+        solve_discr.
+      * eapply eval_mkApps_tCoFix in tv' as [l' [evargs eq]].
+        solve_discr.
+
+    - eapply eval_Const in tv' as [decl' [body' [? ?]]].
+      intuition eauto. eapply IHtv.
+      red in isdecl, H0. rewrite H0 in isdecl. inv isdecl.
+      now rewrite H in H2; inv H2.
+
+    - depelim tv'.
+      * eapply eval_mkApps_tCoFix in tv1 as [l' [evargs eq]].
+        solve_discr.
+      * specialize (IHtv1 _ tv'1). inv IHtv1.
+        solve_discr. inv H.
+        now specialize (IHtv2 _ tv'2).
+      * specialize (IHtv1 _ tv'). solve_discr.
+      * easy.
+
+    - depelim tv'; try easy.
+      * eapply eval_mkApps_tCoFix in tv as [l' [evargs eq]].
+        solve_discr.
+      * specialize (IHtv _ tv'1). solve_discr.
+
+    - depelim tv'; try specialize (IHtv1 _ tv'1); subst; try easy.
+      depelim tv1. easy.
+      specialize (IHtv2 _ tv'2). congruence.
+
+    - depelim tv'; try easy.
+  Qed.
 
 End Wcbv.
